concurrency/scache/CacheIO.i.dfy
@@ -1,0 +1,96 @@
+include "CacheTypes.i.dfy"
+
+module CacheIO(aio: AIO(CacheAIOParams, CacheIfc, CacheSSM)) {
+  import opened CT = CacheTypes(aio)
+  import opened Constants
+  import opened Ptrs
+  import opened NativeTypes
+  import T = RwLockToken
+  import CacheResources
+  import opened CacheAIOParams
+  import opened IocbStruct
+
+  method get_free_io_slot(shared cache: Cache, inout linear local: LocalState)
+  returns (idx: uint64, glinear access: IOSlotAccess)
+  requires cache.Inv()
+  requires old_local.WF()
+  ensures local.WF()
+  ensures 0 <= idx as int < NUM_IO_SLOTS
+  ensures is_slot_access(cache.io_slots[idx], access)
+
+  method disk_writeback_async(
+      shared cache: Cache,
+      inout linear local: LocalState,
+      disk_idx: uint64,
+      cache_idx: uint64,
+      glinear wbo: T.WritebackObtainedToken,
+      glinear ticket: CacheResources.DiskWriteTicket)
+  requires cache.Inv()
+  requires old_local.WF()
+
+  requires 0 <= cache_idx as int < CACHE_SIZE
+  requires 0 <= disk_idx as int < NUM_DISK_PAGES
+  requires wbo.is_handle(cache.key(cache_idx as int))
+  requires wbo.b.CacheEntryHandle?
+  requires ticket == CacheResources.DiskWriteTicket(disk_idx as int, wbo.b.data.s)
+
+  ensures local.WF()
+  {
+    var idx: uint64;
+    glinear var access;
+    idx, access := get_free_io_slot(cache, inout local);
+    glinear var IOSlotAccess(iocb, io_slot_info) := access;
+
+    iocb_prepare_write(
+        cache.io_slots[idx].iocb_ptr,
+        inout iocb,
+        disk_idx as int64,
+        4096,
+        cache.data[cache_idx]);
+
+    cache.io_slots[idx].io_slot_info_ptr.write(
+        inout io_slot_info,
+        IOSlotWrite(cache_idx));
+
+    glinear var writeg := WriteG(
+        cache.key(cache_idx as int),
+        wbo, idx as int, io_slot_info);
+
+    aio.async_write(
+        cache.ioctx,
+        cache.io_slots[idx].iocb_ptr,
+        iocb,
+        wbo.b.data.s,
+        writeg,
+        CacheResources.DiskWriteTicket_unfold(ticket));
+  }
+
+  /*
+  method disk_read_sync(
+      addr: uint64,
+      ptr: Ptr,
+      inout linear contents: ArrayDeref<byte>,
+      linear ticket: DiskReadTicket)
+  returns (linear stub: DiskReadStub)
+  requires |old_contents.s| == 4096
+  requires ticket == DiskReadTicket(addr)
+  requires old_contents.ptr == ptr
+  ensures contents.ptr == ptr
+  ensures |contents.s| == 4096
+  ensures stub == DiskReadStub(addr, contents.s)
+
+
+  method disk_writeback_callback(
+      cache: Cache,
+      addr: uint64,
+      /*readonly*/ linear contents: Ptrs.ArrayDeref<byte>,
+      linear g: CacheIOImpl.WritebackGhostState,
+      linear stub: CacheResources.R)
+  requires cache.Inv()
+  requires stub == CacheResources.DiskWriteStub(addr)
+  requires g.WF(addr)
+  {
+    
+  }
+  */
+}
